Test/Gauss.lean
@@ -1,4 +1,5 @@
 import Test.Gauss.Rec
 import Test.Gauss.SSA
+import Test.Gauss.Simple
 import Test.Monad
 import Test.Peano
